function method

examples/iterators/ElimDup.dfy
@@ -9,45 +9,45 @@ predicate Sorted(xs:seq<int>)
 predicate StrictSorted(xs:seq<int>)
 { forall i,j | 0<=i<j<|xs| :: xs[i]<xs[j]}
  
-function validIt(xs:seq<int>,i:int):bool
-requires 0<=i<=|xs|
-ensures i==0==> validIt(xs,i)
-ensures i==|xs| ==> validIt(xs,i)
-ensures 0<i<|xs| ==> validIt(xs,i)==(xs[i]!=xs[i-1])
+function ValidIt(xs:seq<int>,i:int):bool
+requires -1<=i<=|xs|
+ensures i<=0==> ValidIt(xs,i)
+ensures i==|xs| ==> ValidIt(xs,i)
+ensures 0<i<|xs| ==> ValidIt(xs,i)==(xs[i]!=xs[i-1])
 {
- if (i==0) then true
+ if (i<=0) then true
  else if (i==|xs|) then true
  else xs[i]!=xs[i-1]
 
 }
 
-function delDup(xs:seq<int>,i:int):seq<int>//[0,i)
+function DelDup(xs:seq<int>,i:int):seq<int>//[0,i)
 requires 0<=i<=|xs|
-ensures i==0 ==>delDup(xs,i)==[]
-ensures i==1 ==>delDup(xs,i)==[xs[0]]
-ensures i>1 && xs[i-1]!=xs[i-2] ==> delDup(xs,i)==delDup(xs,i-1)+[xs[i-1]]
-ensures i>1 && xs[i-1]==xs[i-2] ==> delDup(xs,i)==delDup(xs,i-1)
+ensures i==0 ==>DelDup(xs,i)==[]
+ensures i==1 ==>DelDup(xs,i)==[xs[0]]
+ensures i>1 && xs[i-1]!=xs[i-2] ==> DelDup(xs,i)==DelDup(xs,i-1)+[xs[i-1]]
+ensures i>1 && xs[i-1]==xs[i-2] ==> DelDup(xs,i)==DelDup(xs,i-1)
 {
  if (i==0) then []
  else if (i==1) then [xs[0]]
- else if (xs[i-1]!=xs[i-2]) then delDup(xs,i-1)+[xs[i-1]]
- else delDup(xs,i-1)
+ else if (xs[i-1]!=xs[i-2]) then DelDup(xs,i-1)+[xs[i-1]]
+ else DelDup(xs,i-1)
 
 }
 
 
-lemma propDelDupAux(oxs:seq<int>,xs:seq<int>,i:int,j:int)
-requires 0<=i<=|oxs| && 0<=j<= |xs| && xs[..j]==delDup(oxs,i) && xs[j..]==oxs[i..] && Sorted(oxs)
+lemma PropDelDupAux(oxs:seq<int>,xs:seq<int>,i:int,j:int)
+requires 0<=i<=|oxs| && 0<=j<= |xs| && xs[..j]==DelDup(oxs,i) && xs[j..]==oxs[i..] && Sorted(oxs)
  ensures (set x | x in oxs) == (set x | x in xs)
- ensures StrictSorted(xs[..|delDup(oxs,i)|])
+ ensures StrictSorted(xs[..|DelDup(oxs,i)|])
 
 
-lemma propDelDup(oxs:seq<int>,xs:seq<int>)
-requires  xs==delDup(oxs,|oxs|) && Sorted(oxs)
+lemma PropDelDup(oxs:seq<int>,xs:seq<int>)
+requires  xs==DelDup(oxs,|oxs|) && Sorted(oxs)
  ensures (set x | x in oxs) == (set x | x in xs)
- ensures StrictSorted(xs[..|delDup(oxs,|oxs|)|])
+ ensures StrictSorted(xs[..|DelDup(oxs,|oxs|)|])
 
-method elimDup(l:LinkedList<int>)  
+method ElimDup(l:LinkedList<int>)  
  modifies l, l.Repr()
  requires allocated(l.Repr())
  ensures fresh(l.Repr()-old(l.Repr()))
@@ -56,36 +56,38 @@ method elimDup(l:LinkedList<int>)
  requires l.Valid() && Sorted(l.Model())
  ensures l.Valid()
 
- ensures l.Model()==delDup(old(l.Model()),|old(l.Model())|)
+ ensures l.Model()==DelDup(old(l.Model()),|old(l.Model())|)
  ensures (set x | x in old(l.Model())) == (set x | x in l.Model())
  ensures StrictSorted(l.Model())
 
  ensures l.Iterators() >= old(l.Iterators())
- ensures forall it | it in old(l.Iterators()) && old(it.Valid()) && validIt(old(l.Model()),old(it.Index()))
-      ::it.Valid() && it.Parent()==old(it.Parent()) && it.Index()==|delDup(old(l.Model()),old(it.Index()))|
+ ensures forall it | it in old(l.Iterators()) && old(it.Valid()) && ValidIt(old(l.Model()),old(it.Index()))
+      ::it.Valid() && it.Parent()==old(it.Parent()) && 
+      if (old(it.Index()==-1)) then it.Index()==-1
+      else it.Index()==|DelDup(old(l.Model()),old(it.Index()))|
 {
     ghost var validSet:=(set it |it in old(l.Iterators()) && old(it.Valid())::old(it.Index()));
     ghost var omodel:=l.Model();
 
 
-   var it2:=l.Begin(); 
+   var it2:=l.First(); 
    var it1:=it2.Copy();
-   var b := it1.HasNext();
+   var b := it1.HasPeek();
 
    if (b) 
    { 
      
      
-    var _ := it2.Next();
+    it2.Next();
     ghost var j:=1; //to traverse old(l.Model())
     ghost var p:=0;//first occurrence in old(l.Model()) of current element it1
 
-    assert it2.HasNext?() ==> it1.HasNext?() && l.Model()[it1.Index()+1]==l.Model()[it2.Index()];
+    assert it2.HasPeek?() ==> it1.HasPeek?() && l.Model()[it1.Index()+1]==l.Model()[it2.Index()];
     assert it2.Index()==1 && it1.Index()==0;
   
     
 
-    b := it2.HasNext();
+    b := it2.HasPeek();
     while b
      decreases |l.Model()| - it2.Index()
      invariant allocated(l.Repr())
@@ -95,26 +97,32 @@ method elimDup(l:LinkedList<int>)
      invariant it2 in l.Iterators() && it1 in l.Iterators()
      invariant it1.Parent() == l && it2.Parent()==l
      invariant it1.Valid() && it2.Valid()
+     invariant it1.Index() >=0 && it2.Index()>=0
      invariant it2.Index()==it1.Index()+1 
-     invariant it2.HasNext?() ==> it1.HasNext?() && l.Model()[it1.Index()+1]==l.Model()[it2.Index()]
+     invariant it2.HasPeek?() ==> it1.HasPeek?() && l.Model()[it1.Index()+1]==l.Model()[it2.Index()]
      invariant j+(|l.Model()| - it2.Index())==|omodel| && 1<=j<=|old(l.Model())| 
 
-    invariant l.Model()[..it2.Index()]==delDup(old(l.Model()),j)    
+    invariant l.Model()[..it2.Index()]==DelDup(old(l.Model()),j)    
     invariant old(l.Model())[j-1]==l.Model()[it1.Index()]
     invariant l.Model()[it2.Index()..]==old(l.Model())[j..]
     
     invariant forall k | p <= k < j ::old(l.Model())[k]==old(l.Model())[j-1]==l.Model()[it1.Index()]
-    invariant b == it2.HasNext?()
+    invariant b == it2.HasPeek?()
     // invariant (set x | x in old(l.Model())) == (set x | x in l.Model())
     // invariant Sorted(l.Model()) && StrictSorted(l.Model()[..it2.Index()])
 
     invariant l.Iterators() >= old(l.Iterators())
     invariant it1 !in old(l.Iterators()) && it2 !in old(l.Iterators())
-    invariant it2.Index()==|delDup(old(l.Model()),j)|<=j
-    invariant forall it | it in old(l.Iterators()) && old(it.Valid()) && validIt(old(l.Model()),old(it.Index())) && old(it.Index())<j
-         ::it.Valid() && it.Index()==|delDup(old(l.Model()),old(it.Index()))|<it2.Index()
+    invariant it2.Index()==|DelDup(old(l.Model()),j)|<=j
+    invariant forall it | it in old(l.Iterators()) && old(it.Valid()) && ValidIt(old(l.Model()),old(it.Index())) && old(it.Index())<j
+         ::it.Valid() && it.Parent()==old(it.Parent()) &&
+          if (old(it.Index()==-1)) then it.Index()==-1
+          else it.Index()==|DelDup(old(l.Model()),old(it.Index()))|<it2.Index()
+
+         //it.Index()==|DelDup(old(l.Model()),old(it.Index()))|<it2.Index()
     invariant forall it | it in old(l.Iterators()) && old(it.Valid()) && old(it.Index())>=j
-         ::it.Valid() && it.Index()==old(it.Index())-(j-|delDup(old(l.Model()),j)|)
+         ::it.Valid() && it.Parent()==old(it.Parent()) && 
+           it.Index()==old(it.Index())-(j-|DelDup(old(l.Model()),j)|)
    { ghost var pmodel:=l.Model();
 
      var it1Peek := it1.Peek();
@@ -134,31 +142,32 @@ method elimDup(l:LinkedList<int>)
         j:=j+1; 
           
           assert l.Model()==pmodel[..oit2]+pmodel[oit2+1..];
-          assert l.Model()[..it2.Index()]==delDup(old(l.Model()),j);    
+          assert l.Model()[..it2.Index()]==DelDup(old(l.Model()),j);    
         
       }
      else 
        {   
-         assert  old(l.Model())[j]==l.Model()[it2.Index()]!=l.Model()[it1.Index()]==old(l.Model())[j-1];
-         assert l.Model()[it2.Index()..]==[l.Model()[it2.Index()]]+l.Model()[it2.Index()+1..];
-         assert validIt(old(l.Model()),j);
+        assert  old(l.Model())[j]==l.Model()[it2.Index()]!=l.Model()[it1.Index()]==old(l.Model())[j-1];
+        assert l.Model()[it2.Index()..]==[l.Model()[it2.Index()]]+l.Model()[it2.Index()+1..];
+        assert ValidIt(old(l.Model()),j);
 
-         var _ :=it2.Next(); 
-         var _ :=it1.Next();
+        it2.Next(); 
+        it1.Next();
            
-           p:=j;
-           j:=j+1;
-           assert l.Model()[it2.Index()..]==old(l.Model())[j..];
-           assert l.Model()[..it2.Index()]==delDup(old(l.Model()),j);    
+        p:=j;
+        j:=j+1;
+        
+        assert l.Model()[it2.Index()..]==old(l.Model())[j..];
+        assert l.Model()[..it2.Index()]==DelDup(old(l.Model()),j);    
           }
-     b:=it2.HasNext();  
+     b:=it2.HasPeek();  
          
     }
    
     assert j==|old(l.Model())| && it2.Index()==|l.Model()|;
-    assert l.Model()==delDup(old(l.Model()),|old(l.Model())|);
+    assert l.Model()==DelDup(old(l.Model()),|old(l.Model())|);
        //propDelDupAux(old(l.Model()),l.Model(),|old(l.Model())|,|l.Model()|);
-propDelDup(old(l.Model()),l.Model());
+PropDelDup(old(l.Model()),l.Model());
 
    }
    else {
