examples/iterators/ElimDupMap.dfy
@@ -3,120 +3,122 @@ include "../../src/linear/layer2/LinkedList.dfy"
 include "../../src/linear/layer2/ArrayList.dfy"
 
 predicate Sorted(xs:seq<int>)
-{ forall i,j | 0<=i<=j<|xs| :: xs[i]<=xs[j]}
+{ forall i,j | 0 <= i <= j < |xs| :: xs[i] <= xs[j]}
 
 
 predicate StrictSorted(xs:seq<int>)
-{ forall i,j | 0<=i<j<|xs| :: xs[i]<xs[j]}
+{ forall i,j | 0 <= i < j < |xs| :: xs[i] < xs[j]}
  
 
 
-function delDup(xs:seq<int>,i:int):seq<int>//[0,i)
-requires 0<=i<=|xs|
-ensures i==0 ==>delDup(xs,i)==[]
-ensures i==1 ==>delDup(xs,i)==[xs[0]]
-ensures i>1 && xs[i-1]!=xs[i-2] ==> delDup(xs,i)==delDup(xs,i-1)+[xs[i-1]]
-ensures i>1 && xs[i-1]==xs[i-2] ==> delDup(xs,i)==delDup(xs,i-1)
+function DelDup(xs:seq<int>,i:int):seq<int>//[0,i)
+requires 0 <= i <= |xs|
+ensures i==0 ==>DelDup(xs,i)==[]
+ensures i==1 ==>DelDup(xs,i)==[xs[0]]
+ensures i>1 && xs[i-1]!=xs[i-2] ==> DelDup(xs,i)==DelDup(xs,i-1)+[xs[i-1]]
+ensures i>1 && xs[i-1]==xs[i-2] ==> DelDup(xs,i)==DelDup(xs,i-1)
 {
  if (i==0) then []
  else if (i==1) then [xs[0]]
- else if (xs[i-1]!=xs[i-2]) then delDup(xs,i-1)+[xs[i-1]]
- else delDup(xs,i-1)
+ else if (xs[i-1]!=xs[i-2]) then DelDup(xs,i-1)+[xs[i-1]]
+ else DelDup(xs,i-1)
 
 }
 
 
-lemma monotone(xs:seq<int>,i:int,j:int)
-requires 0<=i<j<=|xs|
-ensures |delDup(xs,i)|<|delDup(xs,j)|
+lemma Monotone(xs:seq<int>,i:int,j:int)
+requires 0 <= i < j <= |xs|
+ensures |DelDup(xs,i)| < |DelDup(xs,j)|
 
 
 
-lemma delDupSize(xs:seq<int>,i:int)
-requires 0<=i<=|xs|
-ensures 0<=|delDup(xs,i)|<=i
+lemma DelDupSize(xs:seq<int>,i:int)
+requires 0 <= i <= |xs|
+ensures 0 <= |DelDup(xs,i)| <= i
 {}
 
-function validIt(xs:seq<int>,j:int,it:int):bool
-requires  1<=j<=|xs| && (0<=it<=|xs|)
-ensures it==0 ==> validIt(xs,j,it)==true
-ensures it==|xs| ==> validIt(xs,j,it)==true
-ensures 1<=it<j ==> validIt(xs,j,it)==(xs[it]!=xs[it-1])
-ensures j<=it<|xs| ==>validIt(xs,j,it)==true
-{ ((it==0) || (it==|xs|) || (1<=it<j && (xs[it]!=xs[it-1])) || (j<=it<|xs|)) }
+function ValidIt(xs:seq<int>,j:int,it:int):bool
+requires  1 <= j <= |xs| && (-1 <= it <= |xs|)
+ensures it <= 0 ==> ValidIt(xs,j,it) == true
+ensures it == |xs| ==> ValidIt(xs,j,it) == true
+ensures 1 <= it < j ==> ValidIt(xs,j,it) == (xs[it]!=xs[it-1])
+ensures j <= it <|xs| ==>ValidIt(xs,j,it) == true
+{ ((it <= 0) || (it == |xs|) || (1 <= it < j && (xs[it]!=xs[it-1])) || (j <= it < |xs|)) }
 
-function f(xs:seq<int>,j:int,it:int):int
-requires 1<=j<=|xs| && 0<=it<=|xs|
-ensures it==0 ==> f(xs,j,it)==0
-ensures it>0 && it>=j ==> f(xs,j,it)==it-(j-|delDup(xs,j)|)
-ensures it>0 && it<j ==> f(xs,j,it)==|delDup(xs,it)|
+function Fit(xs:seq<int>,j:int,it:int):int
+requires 1 <= j <= |xs| && -1 <= it <= |xs|
+ensures it <= 0 ==> Fit(xs,j,it)==it
+ensures it>0 && it >= j ==> Fit(xs,j,it)==it-(j-|DelDup(xs,j)|)
+ensures it>0 && it < j ==> Fit(xs,j,it)==|DelDup(xs,it)|
 {
-  if (it==0) then 0
-  else if (it>=j) then it-(j-|delDup(xs,j)|)
-      else |delDup(xs,it)|
+  if (it <= 0) then it
+  else if (it >= j) then it-(j-|DelDup(xs,j)|)
+      else |DelDup(xs,it)|
     
 }
 
-lemma updatef(xs:seq<int>,j:int,it:int)
-requires 1<=j<|xs| && 0<=it<=|xs|
-ensures it==j ==> f(xs,j+1,it)==f(xs,j,it)
-ensures it<j ==> f(xs,j+1,it)==f(xs,j,it)
+lemma Updatef(xs:seq<int>,j:int,it:int)
+requires 1 <= j < |xs| && -1 <= it <= |xs|
+ensures it == j ==> Fit(xs,j+1,it)==Fit(xs,j,it)
+ensures it < j ==> Fit(xs,j+1,it)==Fit(xs,j,it)
 {}
 
 
-function  delMap(xs:seq<int>,its:set<int>,j:int):map<int,int>
-requires 0<=j<=|xs| 
-ensures j==0 ==> delMap(xs,its,j)==map[]
-ensures 1<j<=|xs| ==> forall it | it in delMap(xs,its,j) :: 
-    it in its && 0<=it<=|xs| && validIt(xs,j,it) && delMap(xs,its,j)[it]==f(xs,j,it) 
+function  DelMap(xs:seq<int>,its:set<int>,j:int):map<int,int>
+requires 0 <= j <= |xs| 
+ensures j == 0 ==> DelMap(xs,its,j)==map[]
+ensures 1 < j <= |xs| ==> forall it | it in DelMap(xs,its,j) :: 
+    it in its && -1 <= it <= |xs| && ValidIt(xs,j,it) && DelMap(xs,its,j)[it]==Fit(xs,j,it) 
 { if (j==0) then map[]
-  else map it | it in its && 0<=it<=|xs| && validIt(xs,j,it):: f(xs,j,it)}
+  else map it | it in its && -1<=it<=|xs| && ValidIt(xs,j,it):: Fit(xs,j,it)}
 
 
 
-lemma delMapRange(xs:seq<int>,its:set<int>,j:int)
-requires 0<=j<=|xs| 
- ensures forall it | it in delMap(xs,its,j) && it<j
-       ::delMap(xs,its,j)[it]<|delDup(xs,j)|
- ensures forall it | it in delMap(xs,its,j) && it>j
-       ::delMap(xs,its,j)[it]>|delDup(xs,j)|
-ensures forall it | it in delMap(xs,its,j) && it==j
-       ::delMap(xs,its,j)[it]==|delDup(xs,j)|
+lemma DelMapRange(xs:seq<int>,its:set<int>,j:int)
+requires 0 <= j <= |xs| 
+ ensures forall it | it in DelMap(xs,its,j) && 0 <= it < j
+       ::DelMap(xs,its,j)[it]<|DelDup(xs,j)|
+ ensures forall it | it in DelMap(xs,its,j) && it > j
+       ::DelMap(xs,its,j)[it]>|DelDup(xs,j)|
+ensures forall it | it in DelMap(xs,its,j) && it == j
+       ::DelMap(xs,its,j)[it]==|DelDup(xs,j)|
 {
-forall it | it in delMap(xs,its,j) && it<j
-ensures delMap(xs,its,j)[it]<|delDup(xs,j)|{
- monotone(xs,it,j);
+forall it | it in DelMap(xs,its,j) && 0 <= it < j
+ensures DelMap(xs,its,j)[it]<|DelDup(xs,j)|{
+ Monotone(xs,it,j);
 }
 }
   
 
-lemma updateMapV(xs:seq<int>,its:set<int>,j:int)
-requires 0<j<|xs| 
-ensures   validIt(xs,j+1,j) ==> delMap(xs,its,j+1)==delMap(xs,its,j)
+lemma UpdateMapV(xs:seq<int>,its:set<int>,j:int)
+requires 0 < j < |xs| 
+ensures   ValidIt(xs,j+1,j) ==> DelMap(xs,its,j+1)==DelMap(xs,its,j)
 {
-  if (validIt(xs,j+1,j)){
-    assert |delDup(xs,j+1)|==|delDup(xs,j)|+1;}
+  if (ValidIt(xs,j+1,j)){
+    assert |DelDup(xs,j+1)|==|DelDup(xs,j)|+1;}
 }
 
-lemma updateMapNV(xs:seq<int>,its:set<int>,j:int)
-requires 0<j<|xs| && !validIt(xs,j+1,j)
-ensures forall it | it in delMap(xs,its,j) && it<j :: it in delMap(xs,its,j+1) && delMap(xs,its,j+1)[it]==delMap(xs,its,j)[it]<j
-ensures forall it | it in delMap(xs,its,j) && it>j :: it in delMap(xs,its,j+1) && delMap(xs,its,j+1)[it]==delMap(xs,its,j)[it]-1
-ensures j !in delMap(xs,its,j+1)
+lemma UpdateMapNV(xs:seq<int>,its:set<int>,j:int)
+requires 0 < j < |xs| && !ValidIt(xs,j+1,j)
+ensures forall it | it in DelMap(xs,its,j) && it < j :: it in DelMap(xs,its,j+1) && DelMap(xs,its,j+1)[it]==DelMap(xs,its,j)[it]<j
+ensures forall it | it in DelMap(xs,its,j) && it > j :: it in DelMap(xs,its,j+1) && DelMap(xs,its,j+1)[it]==DelMap(xs,its,j)[it]-1
+ensures j !in DelMap(xs,its,j+1)
 {
-forall it | it in delMap(xs,its,j) && it<j 
-ensures it in delMap(xs,its,j+1) && delMap(xs,its,j+1)[it]==delMap(xs,its,j)[it]<j
+forall it | it in DelMap(xs,its,j) && 0 <= it < j 
+ensures it in DelMap(xs,its,j+1) && DelMap(xs,its,j+1)[it]==DelMap(xs,its,j)[it]<j
 {
-  monotone(xs,it,j);delDupSize(xs,j);
+  Monotone(xs,it,j);DelDupSize(xs,j);
 }
-forall it | it in delMap(xs,its,j) && it>j 
-ensures it in delMap(xs,its,j+1) && delMap(xs,its,j+1)[it]==delMap(xs,its,j)[it]-1
+forall it | it in DelMap(xs,its,j) && it>j 
+ensures it in DelMap(xs,its,j+1) && DelMap(xs,its,j+1)[it]==DelMap(xs,its,j)[it]-1
 {
-  monotone(xs,j,it);delDupSize(xs,j);
-  assert delMap(xs,its,j+1)[it]==it-(j+1-|delDup(xs,j+1)|)==it-(j+1-|delDup(xs,j)|);
+  Monotone(xs,j,it);DelDupSize(xs,j);
+  assert DelMap(xs,its,j+1)[it]==it-(j+1-|DelDup(xs,j+1)|)==it-(j+1-|DelDup(xs,j)|);
 }
 }
-method {:timeLimitMultiplier 100} elimDup(l:LinkedList<int>) returns (ghost mit:map<int,int>)
+
+
+method {:timeLimitMultiplier 100} ElimDup(l:LinkedList<int>) returns (ghost mit:map<int,int>)
 //method elimDupA(l:ArrayList) //NO CHANGES
  modifies l, l.Repr()
  requires allocated(l.Repr())
@@ -126,36 +128,37 @@ method {:timeLimitMultiplier 100} elimDup(l:LinkedList<int>) returns (ghost mit:
  requires l.Valid() && Sorted(l.Model())
  ensures l.Valid()
 
- ensures l.Model()==delDup(old(l.Model()),|old(l.Model())|)
+ ensures l.Model()==DelDup(old(l.Model()),|old(l.Model())|)
  //ensures (set x | x in old(l.Model())) == (set x | x in l.Model())
  //ensures StrictSorted(l.Model())
 
  ensures l.Iterators() >= old(l.Iterators())
- ensures forall it | it in old(l.Iterators()) && old(it.Valid()) && old(it.Index()) in mit::it.Valid() && it.Parent()==old(it.Parent()) && mit[old(it.Index())]==it.Index()
- ensures mit==delMap(old(l.Model()),(set it |it in old(l.Iterators()) && old(it.Valid())::old(it.Index())),|old(l.Model())|)
+ ensures forall it | it in old(l.Iterators()) && old(it.Valid()) && old(it.Index()) in mit::
+  it.Valid() && it.Parent()==old(it.Parent()) && mit[old(it.Index())]==it.Index()
+ ensures mit==DelMap(old(l.Model()),(set it |it in old(l.Iterators()) && old(it.Valid())::old(it.Index())),|old(l.Model())|)
 {
   ghost var validSet:=(set it |it in old(l.Iterators()) && old(it.Valid())::old(it.Index()));
   ghost var omodel:=l.Model();
 
 
-  var it2:=l.Begin(); 
+  var it2:=l.First(); 
   var it1:=it2.Copy();
-  var b := it1.HasNext();
+  var b := it1.HasPeek();
 
   if (b) 
    { 
      
-     mit:=delMap(old(l.Model()),validSet,1);
+     mit:=DelMap(old(l.Model()),validSet,1);
 
-     var _ := it2.Next();
-     ghost var j:=1; //to traverse old(l.Model())
-     ghost var p:=0;//first occurrence in old(l.Model()) of current element it1
+    it2.Next();
+    ghost var j:=1; //to traverse old(l.Model())
+    ghost var p:=0;//first occurrence in old(l.Model()) of current element it1
 
-     assert it2.HasNext?() ==> it1.HasNext?() && l.Model()[it1.Index()+1]==l.Model()[it2.Index()];
+     assert it2.HasPeek?() ==> it1.HasPeek?() && l.Model()[it1.Index()+1]==l.Model()[it2.Index()];
      assert it2.Index()==1 && it1.Index()==0;
   
 
-    b := it2.HasNext();
+    b := it2.HasPeek();
     while b
      decreases |l.Model()| - it2.Index()
      invariant allocated(l.Repr())
@@ -165,22 +168,23 @@ method {:timeLimitMultiplier 100} elimDup(l:LinkedList<int>) returns (ghost mit:
      invariant it2 in l.Iterators() && it1 in l.Iterators()
      invariant it1.Parent() == l && it2.Parent()==l
      invariant it1.Valid() && it2.Valid()
+     invariant it1.Index() >= 0 && it2.Index() >= 0
      invariant it2.Index()==it1.Index()+1 
-     invariant it2.HasNext?() ==> it1.HasNext?() && l.Model()[it1.Index()+1]==l.Model()[it2.Index()]
+     invariant it2.HasPeek?() ==> it1.HasPeek?() && l.Model()[it1.Index()+1]==l.Model()[it2.Index()]
      invariant j+(|l.Model()| - it2.Index())==|omodel| && 1<=j<=|old(l.Model())| 
 
-     invariant l.Model()[..it2.Index()]==delDup(old(l.Model()),j)    
+     invariant l.Model()[..it2.Index()]==DelDup(old(l.Model()),j)    
      invariant old(l.Model())[j-1]==l.Model()[it1.Index()]
      invariant l.Model()[it2.Index()..]==old(l.Model())[j..] 
      invariant forall k | p <= k < j ::old(l.Model())[k]==old(l.Model())[j-1]==l.Model()[it1.Index()]
-     invariant b == it2.HasNext?()
+     invariant b == it2.HasPeek?()
 
      //invariant (set x | x in old(l.Model())) == (set x | x in l.Model())
      //invariant Sorted(l.Model()) && StrictSorted(l.Model()[..it2.Index()])
 
      invariant l.Iterators() >= old(l.Iterators())
      invariant it1 !in old(l.Iterators()) && it2 !in old(l.Iterators())
-     invariant it2.Index()==|delDup(old(l.Model()),j)|<=j
+     invariant it2.Index()==|DelDup(old(l.Model()),j)|<=j
      //invariant forall it | it in old(l.Iterators()) && old(it.Valid()) && old(it.Index())>=j :: it.Index()>=it2.Index();
      //invariant forall it | it in old(l.Iterators()) && old(it.Valid()) && it.Valid() && it.Index()>it2.Index() :: old(it.Index())>j;
 
@@ -190,10 +194,10 @@ method {:timeLimitMultiplier 100} elimDup(l:LinkedList<int>) returns (ghost mit:
      //   ::mit[old(it.Index())]<it2.Index()
      //invariant forall it | it in old(l.Iterators()) && old(it.Valid()) && old(it.Index()) in mit && old(it.Index())>=j
      //   ::mit[old(it.Index())]>=it2.Index()
-     invariant mit==delMap(old(l.Model()),(set it |it in old(l.Iterators()) && old(it.Valid())::old(it.Index())),j)
+     invariant mit==DelMap(old(l.Model()),(set it |it in old(l.Iterators()) && old(it.Valid())::old(it.Index())),j)
    { ghost var pmodel:=l.Model();
      
-       assert  j in mit ==> mit[j]==|delDup(old(l.Model()),j)|;
+       assert  j in mit ==> mit[j]==|DelDup(old(l.Model()),j)|;
      
      var it1Peek := it1.Peek();
      var it2Peek := it2.Peek();
@@ -205,68 +209,69 @@ method {:timeLimitMultiplier 100} elimDup(l:LinkedList<int>) returns (ghost mit:
         ghost var oit2:=it2.Index();
           
         assert it2 !in old(l.Iterators()); 
-        assert j<j+1 && old(l.Model())[j]==old(l.Model())[j-1];
-        assert !validIt(old(l.Model()),j+1,j);
+        assert j < j+1 && old(l.Model())[j]==old(l.Model())[j-1];
+        assert !ValidIt(old(l.Model()),j+1,j);
         
-        delMapRange(old(l.Model()),validSet,j);     
+        DelMapRange(old(l.Model()),validSet,j);     
         
-      it2 := l.Erase(it2);  
+        it2 := l.Erase(it2);  
           
         assert forall it | it in old(l.Iterators()) && old(it.Valid()) && old(it.Index()) in mit && old(it.Index()) <j
           ::it.Valid() && mit[old(it.Index())]==it.Index()<j;
         assert forall it | it in old(l.Iterators()) && old(it.Valid()) && old(it.Index()) in mit && old(it.Index()) >j
           ::it.Valid() && mit[old(it.Index())]==it.Index()+1;
-        updateMapNV(old(l.Model()),validSet,j);
+        UpdateMapNV(old(l.Model()),validSet,j);
      
 
-      j:=j+1;
+        j:=j+1;
 
         assert l.Model()==pmodel[..oit2]+pmodel[oit2+1..];
-        assert l.Model()[..it2.Index()]==delDup(old(l.Model()),j);    
+        assert l.Model()[..it2.Index()]==DelDup(old(l.Model()),j);    
        
-        mit:=delMap(old(l.Model()),validSet,j);
+        mit:=DelMap(old(l.Model()),validSet,j);
 
          
         assert forall it | it in old(l.Iterators()) && old(it.Valid()) && old(it.Index()) in mit::it.Valid() && mit[old(it.Index())]==it.Index();
-        assert mit==delMap(old(l.Model()),validSet,j);
+        assert mit==DelMap(old(l.Model()),validSet,j);
         assert l.Model()[it2.Index()..]==old(l.Model())[j..];
 
 
-    }
-  else 
-  {   
-      assert  old(l.Model())[j]==l.Model()[it2.Index()]!=l.Model()[it1.Index()]==old(l.Model())[j-1];
-      assert l.Model()[it2.Index()..]==[l.Model()[it2.Index()]]+l.Model()[it2.Index()+1..];
+      }
+    else 
+     {   
+        assert  old(l.Model())[j]==l.Model()[it2.Index()]!=l.Model()[it1.Index()]==old(l.Model())[j-1];
+        assert l.Model()[it2.Index()..]==[l.Model()[it2.Index()]]+l.Model()[it2.Index()+1..];
 
 
-      assert validIt(old(l.Model()),j+1,j);
-      updateMapV(old(l.Model()),validSet,j);
-      assert delMap(old(l.Model()),validSet,j+1)==delMap(old(l.Model()),validSet,j);
+        assert ValidIt(old(l.Model()),j+1,j);
+        UpdateMapV(old(l.Model()),validSet,j);
+        assert DelMap(old(l.Model()),validSet,j+1)==DelMap(old(l.Model()),validSet,j);
       
-      var _ := it2.Next(); 
-      var _ := it1.Next();
+        it2.Next(); 
+        it1.Next();
            
-      p:=j;
-      j:=j+1;
-      assert l.Model()[it2.Index()..]==old(l.Model())[j..];
-      assert l.Model()[..it2.Index()]==delDup(old(l.Model()),j); 
+        p:=j;
+        j:=j+1;
+      
+        assert l.Model()[it2.Index()..]==old(l.Model())[j..];
+        assert l.Model()[..it2.Index()]==DelDup(old(l.Model()),j); 
 
-      mit:=delMap(old(l.Model()),validSet,j);
-      assert forall it | it in old(l.Iterators()) && old(it.Valid()) && old(it.Index()) in mit::it.Valid() && mit[old(it.Index())]==it.Index();
-      assert mit==delMap(old(l.Model()),validSet,j);
+        mit:=DelMap(old(l.Model()),validSet,j); 
+        assert forall it | it in old(l.Iterators()) && old(it.Valid()) && old(it.Index()) in mit::
+         it.Valid() && it.Parent()==old(it.Parent()) && mit[old(it.Index())]==it.Index();
+        assert mit==DelMap(old(l.Model()),validSet,j);
+      }
+    b:=it2.HasPeek();  
   }
-  b:=it2.HasNext();  
-
-}
-    assert mit==delMap(old(l.Model()),validSet,j);
-    assert j==|old(l.Model())| && it2.Index()==|l.Model()|;
-    assert l.Model()==delDup(old(l.Model()),|old(l.Model())|);
+  assert mit==DelMap(old(l.Model()),validSet,j);
+  assert j==|old(l.Model())| && it2.Index()==|l.Model()|;
+  assert l.Model()==DelDup(old(l.Model()),|old(l.Model())|);
 
 
-    //assert forall it | it in old(l.Iterators()) && old(it.Valid()) && old(it.Index()) in mit::it.Valid() && mit[old(it.Index())]==it.Index();
+  //assert forall it | it in old(l.Iterators()) && old(it.Valid()) && old(it.Index()) in mit::it.Valid() && mit[old(it.Index())]==it.Index();
    }
-   else {
+  else {
          mit:=map[];
        }
 
-   }
+}
