src/Order.dfy
@@ -1,42 +1,44 @@
-predicate isPreorder<A(!new)>(le: (A, A) -> bool)
+predicate IsPreorder<A(!new)>(le: (A, A) -> bool)
 {
   (forall a :: le(a, a)) &&
   (forall a, b, c | le(a, b) && le(b, c) :: le(a, c))
 }
 
-predicate isTotalPreorder<A(!new)>(le: (A, A) -> bool)
+predicate IsTotalPreorder<A(!new)>(le: (A, A) -> bool)
 {
-  isPreorder(le) &&
+  IsPreorder(le) &&
   (forall a, b :: le(a, b) || le(b, a))
 }
 
-predicate isPartialOrder<A(!new)>(le: (A, A) -> bool)
+predicate IsPartialOrder<A(!new)>(le: (A, A) -> bool)
 {
   (forall a :: le(a, a)) &&
   (forall a, b | le(a, b) && le(b, a) :: a == b) &&
   (forall a, b, c | le(a, b) && le(b, c) :: le(a, c))
 }
 
-predicate isTotalOrder<A(!new)>(le: (A, A) -> bool)
+predicate IsTotalOrder<A(!new)>(le: (A, A) -> bool)
 {
-  isTotalPreorder(le) &&
+  IsTotalPreorder(le) &&
   (forall a, b | le(a, b) && le(b, a) :: a == b)
 }
 
-lemma partialOrderAndTotalPreorder<A(!new)>(le: (A, A) -> bool)
-  requires isTotalPreorder(le)
-  requires isPartialOrder(le)
-  ensures isTotalOrder(le)
+lemma PartialOrderAndTotalPreorder<A(!new)>(le: (A, A) -> bool)
+  requires IsTotalPreorder(le)
+  requires IsPartialOrder(le)
+  ensures IsTotalOrder(le)
 {
 }
 
 predicate Ordered<A>(xs: seq<A>, le: (A, A) -> bool)
-  requires isTotalOrder(le)
+  requires IsTotalOrder(le)
 {
-  forall i | 0 <= i < |xs|-1 :: le(xs[i], xs[i+1])
+  forall i, j | 0 <= i < j < |xs| :: le(xs[i], xs[j])
 }
 
 predicate OrderedInt(xs: seq<int>)
 {
-  forall i, j | 0 <= i < j < |xs| :: xs[i] < xs[j]
+  //forall i, j | 0 <= i < j < |xs| :: xs[i] < xs[j]
+  Ordered<int>(xs,(x,y) => x<= y)
 }
+
